<?xml version="1.0"?>


<!DOCTYPE rdf:RDF [
    <!ENTITY owl "http://www.w3.org/2002/07/owl#" >
    <!ENTITY xsd "http://www.w3.org/2001/XMLSchema#" >
    <!ENTITY rdfs "http://www.w3.org/2000/01/rdf-schema#" >
    <!ENTITY rdf "http://www.w3.org/1999/02/22-rdf-syntax-ns#" >
    <!ENTITY dc "http://purl.org/dc/elements/1.1/" >
]>


<rdf:RDF xmlns="http://purl.org/ceu/errors/"
     xml:base="http://purl.org/ceu/errors/"
     xmlns:rdf="http://www.w3.org/1999/02/22-rdf-syntax-ns#"
     xmlns:owl="http://www.w3.org/2002/07/owl#"
     xmlns:xsd="http://www.w3.org/2001/XMLSchema#"
     xmlns:rdfs="http://www.w3.org/2000/01/rdf-schema#"
     xmlns:dc="http://purl.org/dc/elements/1.1/">
    <owl:Ontology rdf:about="http://purl.org/ceu/errors/">
        <rdfs:label xml:lang="en">Errors ontology</rdfs:label>
        <rdfs:comment xml:lang="en">The Errors ontology, is an ontology for tracking semantic inconsistencies an modelling errors in ontologies.</rdfs:comment>
        <rdfs:comment xml:lang="es">La ontología Errors es una ontología para registrar inconsistencias semánticas y errores de modelado en ontologías.</rdfs:comment>
        <owl:versionIRI rdf:resource="http://purl.org/ceu/errors/1.0"/>
        <dc:creator xml:lang="es">Alfredo Sánchez Alberca (asalber@ceu.es) &lt;http://aprendeconalf.es/foaf.rdf&gt;</dc:creator>
        <dc:rights xml:lang="en">E-Collections ontology is released under Attribution-ShareAlike 4.0 International Creative Commons license: http://creativecommons.org/licenses/by-sa/4.0/</dc:rights>
        <dc:rights xml:lang="es">La ontología E-Collections está bajo una licencia de Creative Commons Reconocimiento-CompartirIgual 4.0 Internacional ( http://creativecommons.org/licenses/by-sa/4.0/).</dc:rights>
    </owl:Ontology>
    


    <!-- 
    ///////////////////////////////////////////////////////////////////////////////////////
    //
    // Object Properties
    //
    ///////////////////////////////////////////////////////////////////////////////////////
     -->

    


    <!-- http://purl.org/ceu/errors/hasError -->

    <owl:ObjectProperty rdf:about="http://purl.org/ceu/errors/hasError">
        <rdfs:label xml:lang="en">has error</rdfs:label>
        <rdfs:label xml:lang="es">tiene error</rdfs:label>
        <rdfs:comment xml:lang="en">Property that relates an entity with an inconsistent definition or a semantic error (which results in it belonging to the class owl:Nothing, therefore making the model inconsistent) to an error.</rdfs:comment>
        <rdfs:comment xml:lang="es">Propiedad que relaciona una entidad con una definición inconsistente o con un error semántico con un error.</rdfs:comment>
        <rdfs:range rdf:resource="http://purl.org/ceu/errors/Error"/>
        <rdfs:domain>
            <owl:Restriction>
                <owl:onProperty rdf:resource="http://purl.org/ceu/errors/hasError"/>
                <owl:onClass rdf:resource="http://purl.org/ceu/errors/Error"/>
                <owl:qualifiedCardinality rdf:datatype="&xsd;nonNegativeInteger">0</owl:qualifiedCardinality>
            </owl:Restriction>
        </rdfs:domain>
    </owl:ObjectProperty>
    


    <!-- 
    ///////////////////////////////////////////////////////////////////////////////////////
    //
    // Data properties
    //
    ///////////////////////////////////////////////////////////////////////////////////////
     -->

    


    <!-- http://purl.org/ceu/errors/errorDescription -->

    <owl:DatatypeProperty rdf:about="http://purl.org/ceu/errors/errorDescription">
        <rdfs:label xml:lang="en">error description</rdfs:label>
        <rdfs:label xml:lang="es">descripción del error</rdfs:label>
        <rdfs:comment xml:lang="en">Property that relates an error with a textual description of the error.</rdfs:comment>
        <rdfs:comment xml:lang="es">Propiedad que relaciona un error con una descripción textual del error.</rdfs:comment>
    </owl:DatatypeProperty>
    


    <!-- 
    ///////////////////////////////////////////////////////////////////////////////////////
    //
    // Classes
    //
    ///////////////////////////////////////////////////////////////////////////////////////
     -->

    


    <!-- http://purl.org/ceu/errors/CardinalityError -->

    <owl:Class rdf:about="http://purl.org/ceu/errors/CardinalityError">
        <rdfs:label xml:lang="en">Cardinality error</rdfs:label>
        <rdfs:label xml:lang="es">Error de cardinalidad</rdfs:label>
        <rdfs:subClassOf rdf:resource="http://purl.org/ceu/errors/CollectionError"/>
    </owl:Class>
    


    <!-- http://purl.org/ceu/errors/CollectionError -->

    <owl:Class rdf:about="http://purl.org/ceu/errors/CollectionError">
        <rdfs:label xml:lang="en">Collection error</rdfs:label>
        <rdfs:label xml:lang="es">Error de colección</rdfs:label>
        <rdfs:subClassOf rdf:resource="http://purl.org/ceu/errors/Error"/>
    </owl:Class>
    


    <!-- http://purl.org/ceu/errors/Error -->

    <owl:Class rdf:about="http://purl.org/ceu/errors/Error">
        <rdfs:label xml:lang="en">Error</rdfs:label>
        <rdfs:label xml:lang="es">Error</rdfs:label>
        <rdfs:comment xml:lang="en">A semantic error in an inconsistent ontology.</rdfs:comment>
        <rdfs:comment xml:lang="es">Un error semántico en una ontología inconsistente.</rdfs:comment>
    </owl:Class>
    


    <!-- http://purl.org/ceu/errors/HomogeneityError -->

    <owl:Class rdf:about="http://purl.org/ceu/errors/HomogeneityError">
        <rdfs:label xml:lang="en">Homogeneity error</rdfs:label>
        <rdfs:label xml:lang="es">Error de homogeneidad</rdfs:label>
        <rdfs:subClassOf rdf:resource="http://purl.org/ceu/errors/CollectionError"/>
    </owl:Class>
    


    <!-- http://purl.org/ceu/errors/OrderError -->

    <owl:Class rdf:about="http://purl.org/ceu/errors/OrderError">
        <rdfs:label xml:lang="en">Order error</rdfs:label>
        <rdfs:label xml:lang="es">Error de orden</rdfs:label>
        <rdfs:subClassOf rdf:resource="http://purl.org/ceu/errors/CollectionError"/>
    </owl:Class>
    


    <!-- http://purl.org/ceu/errors/UniquenessError -->

    <owl:Class rdf:about="http://purl.org/ceu/errors/UniquenessError">
        <rdfs:label xml:lang="en">Uniqueness error</rdfs:label>
        <rdfs:label xml:lang="es">Error de unicidad</rdfs:label>
        <rdfs:subClassOf rdf:resource="http://purl.org/ceu/errors/CollectionError"/>
    </owl:Class>
</rdf:RDF>



<!-- Generated by the OWL API (version 3.5.1) http://owlapi.sourceforge.net -->

