Prefix(:=<http://purl.org/ceu/errors/>)
Prefix(dc:=<http://purl.org/dc/elements/1.1/>)
Prefix(owl:=<http://www.w3.org/2002/07/owl#>)
Prefix(rdf:=<http://www.w3.org/1999/02/22-rdf-syntax-ns#>)
Prefix(xml:=<http://www.w3.org/XML/1998/namespace>)
Prefix(xsd:=<http://www.w3.org/2001/XMLSchema#>)
Prefix(rdfs:=<http://www.w3.org/2000/01/rdf-schema#>)


Ontology(<http://purl.org/ceu/errors/>
<http://purl.org/ceu/errors/1.0>
Annotation(dc:creator "Alfredo Sánchez Alberca (asalber@ceu.es) <http://aprendeconalf.es/foaf.rdf>"@es)
Annotation(rdfs:comment "La ontología Errors es una ontología para registrar inconsistencias semánticas y errores de modelado en ontologías."@es)
Annotation(rdfs:comment "The Errors ontology, is an ontology for tracking semantic inconsistencies an modelling errors in ontologies."@en)
Annotation(dc:rights "Errors ontology is released under Attribution-ShareAlike 4.0 International Creative Commons license: http://creativecommons.org/licenses/by-sa/4.0/"@en)
Annotation(dc:rights "La ontología Errors está bajo una licencia de Creative Commons Reconocimiento-CompartirIgual 4.0 Internacional ( http://creativecommons.org/licenses/by-sa/4.0/)."@es)
Annotation(rdfs:label "Errors ontology"@en)

Declaration(Class(:CardinalityError))
Declaration(Class(:CollectionError))
Declaration(Class(:Error))
Declaration(Class(:HomogeneityError))
Declaration(Class(:OrderError))
Declaration(Class(:UniquenessError))
Declaration(ObjectProperty(:hasError))
Declaration(DataProperty(:errorDescription))
AnnotationAssertion(rdfs:label :CardinalityError "Cardinality error"@en)
AnnotationAssertion(rdfs:label :CardinalityError "Error de cardinalidad"@es)
SubClassOf(:CardinalityError :CollectionError)
AnnotationAssertion(rdfs:label :CollectionError "Collection error"@en)
AnnotationAssertion(rdfs:label :CollectionError "Error de colección"@es)
SubClassOf(:CollectionError :Error)
AnnotationAssertion(rdfs:label :Error "Error"@es)
AnnotationAssertion(rdfs:comment :Error "Un error semántico en una ontología inconsistente."@es)
AnnotationAssertion(rdfs:comment :Error "A semantic error in an inconsistent ontology."@en)
AnnotationAssertion(rdfs:label :Error "Error"@en)
AnnotationAssertion(rdfs:label :HomogeneityError "Error de homogeneidad"@es)
AnnotationAssertion(rdfs:label :HomogeneityError "Homogeneity error"@en)
SubClassOf(:HomogeneityError :CollectionError)
AnnotationAssertion(rdfs:label :OrderError "Order error"@en)
AnnotationAssertion(rdfs:label :OrderError "Error de orden"@es)
SubClassOf(:OrderError :CollectionError)
AnnotationAssertion(rdfs:label :UniquenessError "Uniqueness error"@en)
AnnotationAssertion(rdfs:label :UniquenessError "Error de unicidad"@es)
SubClassOf(:UniquenessError :CollectionError)
AnnotationAssertion(rdfs:comment :hasError "Property that relates an entity with an inconsistent definition or a semantic error (which results in it belonging to the class owl:Nothing, therefore making the model inconsistent) to an error."@en)
AnnotationAssertion(rdfs:label :hasError "has error"@en)
AnnotationAssertion(rdfs:comment :hasError "Propiedad que relaciona una entidad con una definición inconsistente o con un error semántico con un error."@es)
AnnotationAssertion(rdfs:label :hasError "tiene error"@es)
ObjectPropertyDomain(:hasError ObjectExactCardinality(0 :hasError :Error))
ObjectPropertyRange(:hasError :Error)
AnnotationAssertion(rdfs:comment :errorDescription "Property that relates an error with a textual description of the error."@en)
AnnotationAssertion(rdfs:comment :errorDescription "Propiedad que relaciona un error con una descripción textual del error."@es)
AnnotationAssertion(rdfs:label :errorDescription "error description"@en)
AnnotationAssertion(rdfs:label :errorDescription "descripción del error"@es)
)